Support for statics

case_studies/tests/src/statics.rs
@@ -1,0 +1,9 @@
+
+#[rr::name("MYINT")]
+static MYINT: i32 = 42;
+
+#[rr::requires(#iris "initialized π \"MYINT\" 42")]
+#[rr::returns("42")]
+fn read_static_1() -> i32 {
+    MYINT
+}
