rr_frontend/translation/src/spec_parsers/const_attr_parser.rs
@@ -1,0 +1,79 @@
+// © 2023, The RefinedRust Developers and Contributors
+//
+// This Source Code Form is subject to the terms of the BSD-3-clause License.
+// If a copy of the BSD-3-clause license was not distributed with this
+// file, You can obtain one at https://opensource.org/license/bsd-3-clause/.
+
+use attribute_parse as parse;
+use radium::specs;
+use rustc_ast::ast::AttrItem;
+use rustc_hir::def_id::{DefId, LocalDefId};
+
+use crate::spec_parsers::parse_utils;
+
+/// Parse attributes on a const.
+/// Permitted attributes:
+/// - rr::name("x"), which will introduce the name x to refer to the const in other specs
+pub trait ConstAttrParser {
+    fn parse_const_attrs<'a>(
+        &'a mut self,
+        did: LocalDefId,
+        attrs: &'a [&'a AttrItem],
+    ) -> Result<ConstAttrs, String>;
+}
+
+#[derive(Debug, Clone)]
+pub struct ConstAttrs {
+    pub name: String,
+}
+
+pub struct VerboseConstAttrParser {}
+
+impl VerboseConstAttrParser {
+    pub fn new() -> Self {
+        VerboseConstAttrParser {}
+    }
+}
+
+impl ConstAttrParser for VerboseConstAttrParser {
+    fn parse_const_attrs<'a>(
+        &'a mut self,
+        _did: LocalDefId,
+        attrs: &'a [&'a AttrItem],
+    ) -> Result<ConstAttrs, String> {
+        fn str_err(e: parse::ParseError) -> String {
+            format!("{:?}", e)
+        }
+
+        let meta = ();
+        let mut name: Option<String> = None;
+
+        for &it in attrs.iter() {
+            let ref path_segs = it.path.segments;
+            let ref args = it.args;
+
+            if let Some(seg) = path_segs.get(1) {
+                let buffer = parse::ParseBuffer::new(&it.args.inner_tokens());
+                match &*seg.ident.name.as_str() {
+                    "name" => {
+                        let parsed_name: parse::LitStr = buffer.parse(&meta).map_err(str_err)?;
+                        if name.is_some() {
+                            return Err(format!("name attribute has already been specified"));
+                        }
+                        name = Some(parsed_name.value());
+                    },
+                    _ => {
+                        return Err(format!("unknown attribute for const specification: {:?}", args));
+                    },
+                }
+            }
+        }
+        if name.is_none() {
+            Err(format!("no name attribute specified on const"))
+        } else {
+            Ok(ConstAttrs {
+                name: name.unwrap(),
+            })
+        }
+    }
+}
