stdlib/spin/theories/once/once_ghost_state.v
@@ -19,20 +19,13 @@ Section once.
   Context `{onceG Σ A}.
 
   Definition once_uninit_tok_def γ := own γ (Cinl (1/2)%Qp).
-  Definition once_uninit_tok_aux : seal (@once_uninit_tok_def). Proof. by eexists. Qed.
-  Definition once_uninit_tok := once_uninit_tok_aux.(unseal).
-  Definition once_uninit_tok_eq : @once_uninit_tok = @once_uninit_tok_def := once_uninit_tok_aux.(seal_eq).
-
 
   Definition once_init_tok_def γ (a : A) := own γ (Cinr (to_agree (a : leibnizO A))).
-  Definition once_init_tok_aux : seal (@once_init_tok_def). Proof. by eexists. Qed.
-  Definition once_init_tok := once_init_tok_aux.(unseal).
-  Definition once_init_tok_eq : @once_init_tok = @once_init_tok_def := once_init_tok_aux.(seal_eq).
 
   Definition once_status_tok_def γ (a : option A) :=
     match a with
-    | None => once_uninit_tok γ
-    | Some a => once_init_tok γ a
+    | None => once_uninit_tok_def γ
+    | Some a => once_init_tok_def γ a
     end.
   Definition once_status_tok_aux : seal (@once_status_tok_def). Proof. by eexists. Qed.
   Definition once_status_tok := once_status_tok_aux.(unseal).
@@ -40,18 +33,18 @@ Section once.
 
 
   Lemma once_uninit_tok_alloc :
-    ⊢ |==> ∃ γ, once_uninit_tok γ ∗ once_uninit_tok γ.
+    ⊢ |==> ∃ γ, once_status_tok γ None ∗ once_status_tok γ None.
   Proof.
-    rewrite once_uninit_tok_eq /once_uninit_tok_def. 
+    rewrite once_status_tok_eq /once_status_tok_def.
     setoid_rewrite <-own_op.
     rewrite -Cinl_op frac_op Qp.half_half.
     iApply own_alloc. done.
   Qed.
 
   Lemma once_uninit_tok_init γ a :
-    once_uninit_tok γ -∗ once_uninit_tok γ -∗ |==> once_init_tok γ a.
+    once_status_tok γ None -∗ once_status_tok γ None -∗ |==> once_status_tok γ (Some a).
   Proof.
-    rewrite once_uninit_tok_eq once_init_tok_eq.
+    rewrite once_status_tok_eq.
     iIntros "Ha Hb".
     iCombine "Ha Hb" as "Ha".
     rewrite -Cinl_op frac_op Qp.half_half.
@@ -59,114 +52,74 @@ Section once.
     by apply cmra_update_exclusive.
   Qed.
 
-  Global Instance once_init_tok_persistent γ a : Persistent (once_init_tok γ a).
-  Proof. rewrite once_init_tok_eq. apply _. Qed.
   Global Instance once_status_tok_persistent γ a : Persistent (once_status_tok γ (Some a)).
   Proof. rewrite once_status_tok_eq. apply _. Qed.
 
   Lemma once_uninit_init_tok_False γ a :
-    once_uninit_tok γ -∗ once_init_tok γ a -∗ False.
+    once_status_tok γ None -∗ once_status_tok γ (Some a) -∗ False.
   Proof.
-    iIntros "H1 H2". rewrite once_uninit_tok_eq once_init_tok_eq.
+    iIntros "H1 H2". rewrite once_status_tok_eq.
     iDestruct (own_valid_2 with "H1 H2") as %Hv.
     done.
   Qed.
 
   Lemma once_uninit_uninit_tok_False γ :
-    once_uninit_tok γ -∗ once_uninit_tok γ -∗ once_uninit_tok γ -∗ False.
+    once_status_tok γ None -∗ once_status_tok γ None -∗ once_status_tok γ None -∗ False.
   Proof.
-    iIntros "H1 H2 H3". rewrite once_uninit_tok_eq.
+    iIntros "H1 H2 H3". rewrite once_status_tok_eq.
     iDestruct (own_valid_3 with "H1 H2 H3") as %Hv.
     done.
   Qed.
 
   Lemma once_init_tok_agree γ a b :
-    once_init_tok γ a -∗ once_init_tok γ b -∗ ⌜a = b⌝.
+    once_status_tok γ (Some a) -∗ once_status_tok γ (Some b) -∗ ⌜a = b⌝.
   Proof.
-    iIntros "H1 H2". rewrite once_init_tok_eq.
+    iIntros "H1 H2". rewrite once_status_tok_eq.
     iDestruct (own_valid_2 with "H1 H2") as %Hv.
     iPureIntro. by apply to_agree_op_inv_L in Hv.
   Qed.
 
-  Global Instance once_init_tok_timeless γ a : Timeless (once_init_tok γ a).
-  Proof. rewrite once_init_tok_eq. apply _. Qed.
-  Global Instance once_uninit_tok_timeless γ : Timeless (once_uninit_tok γ).
-  Proof. rewrite once_uninit_tok_eq. apply _. Qed.
+  Global Instance once_init_tok_timeless γ a : Timeless (once_status_tok γ a).
+  Proof. rewrite once_status_tok_eq; destruct a; apply _. Qed.
 End once.
+
+Notation once_uninit_tok γ := (once_status_tok γ None).
+Notation once_init_tok γ a := (once_status_tok γ (Some a)).
 
 Section typing.
   Context {A} `{!typeGS Σ} `{!onceG Σ A}.
 
-  Lemma subsume_once_status γ a b T :
+  Lemma subsume_once_status_tok γ a b T :
     subsume (once_status_tok γ a) (once_status_tok γ b) T :-
       exhale ⌜a = b⌝; return T.
   Proof.
     iIntros "(-> & HT)".
     iIntros "$"; done.
   Qed.
-  Definition subsume_once_status_inst := [instance subsume_once_status].
-  Global Existing Instance subsume_once_status_inst.
+  Definition subsume_once_status_tok_inst := [instance subsume_once_status_tok].
+  Global Existing Instance subsume_once_status_tok_inst.
 
-  Definition FindOnceStatus γ : find_in_context_info :=
+  Definition FindOnceStatusTok γ : find_in_context_info :=
     {| fic_A := option A; fic_Prop a := once_status_tok γ a |}.
-  Global Instance once_status_related γ a : RelatedTo (once_status_tok γ a) := {| rt_fic := FindOnceStatus γ |}.
+  Global Instance once_status_tok_related γ a : RelatedTo (once_status_tok γ a) := {| rt_fic := FindOnceStatusTok γ |}.
+End typing.
 
-  (*
-  Lemma subsume_once_init γ a b T :
-    subsume (once_init_tok γ a) (once_init_tok γ b) T :-
+(** Since a frequent use case of once is in conjunction with static variables, we provide some extra support for that *)
+Section statics.
+  Context {A} `{!typeGS Σ} `{!staticGS Σ} `{!onceG Σ A}.
+
+  Definition once_status π (s : string) (a : option A) : iProp Σ :=
+    ∃ γ, once_status_tok γ a ∗ initialized π s γ.
+  Global Typeclasses Opaque once_status.
+
+  Definition FindOnceStatus π s : find_in_context_info :=
+    {| fic_A := option A; fic_Prop a := once_status π s a |}.
+  Global Instance once_status_related π s a : RelatedTo (once_status π s a) := {| rt_fic := FindOnceStatus π s |}.
+  Lemma subsume_once_status π s a b T :
+    subsume (once_status π s a) (once_status π s b) T :-
       exhale ⌜a = b⌝; return T.
   Proof.
     iIntros "(-> & HT)".
     iIntros "$"; done.
   Qed.
-  Definition subsume_once_init_inst := [instance subsume_once_init].
-  Global Existing Instance subsume_once_init_inst.
-
-  Lemma subsume_once_init_status γ a b T :
-    subsume (once_init_tok γ a) (once_status_tok γ b) T :-
-      exhale ⌜b = Some a⌝; return T.
-  Proof.
-    iIntros "(-> & HT)".
-    rewrite once_status_tok_eq/=.
-    iIntros "$"; done.
-  Qed.
-  Definition subsume_once_init_status_inst := [instance subsume_once_init_status].
-  Global Existing Instance subsume_once_init_status_inst.
-
-  Lemma subsume_once_uninit γ T :
-    subsume (once_uninit_tok γ) (once_uninit_tok γ) T :-
-      return T.
-  Proof.
-    iIntros "HT $"; done.
-  Qed.
-  Definition subsume_once_uninit_inst := [instance subsume_once_uninit].
-  Global Existing Instance subsume_once_uninit_inst.
-
-  Lemma subsume_once_uninit_status γ b T :
-    subsume (once_uninit_tok γ) (once_status_tok γ b) T :-
-      exhale ⌜b = None⌝; return T.
-  Proof.
-    iIntros "(-> & HT)".
-    rewrite once_status_tok_eq/=.
-    iIntros "$"; done.
-  Qed.
-  Definition subsume_once_uninit_status_inst := [instance subsume_once_uninit_status].
-  Global Existing Instance subsume_once_uninit_status_inst.
-
-  Definition FindOnceInit γ : find_in_context_info :=
-    {| fic_A := A; fic_Prop a := once_init_tok γ a |}.
-  Global Instance once_init_related γ a : RelatedTo (once_init_tok γ a) := {| rt_fic := FindOnceInit γ |}.
-
-  Definition FindOnceUninit γ : find_in_context_info :=
-    {| fic_A := unit; fic_Prop a := once_uninit_tok γ |}.
-  Global Instance once_uninit_related γ : RelatedTo (once_uninit_tok γ) := {| rt_fic := FindOnceUninit γ |}.
-
-  Definition simplify_hyp_once_status_init :
-    simplify_hyp
-    *)
-
-  (* TODO: first add infrastructure for associating ghost state with locations
-  Definition once_status (l : loc) (x : option A) :=
-    ∃ γ, ghost_loc_map l γ ∗ once_status_tok γ x.
-   *)
-End typing.
+End statics.
