theories/rust_typing/static.v
@@ -1,0 +1,106 @@
+From refinedrust Require Import base type ltypes programs references.
+From iris.base_logic Require Import ghost_map.
+
+(* TODO: should require that type is Send? *)
+Class staticGS `{!typeGS Σ} := {
+  static_locs : gmap string loc;
+  static_types : gmap string (sigT type);
+}.
+Global Arguments staticGS _ {_}.
+
+
+Section statics.
+  Context `{!typeGS Σ} `{!staticGS Σ}.
+
+  (** Assertion stating that the static with name [x] has been registered for location [l] and type [ty]. *)
+  (** We assume registration for the expected type and the location parameter in the context where we verify our code *)
+  Definition static_is_registered (x : string) (l : loc) (ty : sigT type) :=
+    static_locs !! x = Some l ∧ static_types !! x = Some ty.
+
+  Import EqNotations.
+
+  (* The global variable "name" has been initialized with refinement "r" *)
+  Definition initialized {rt} (π : thread_id) (name : string) (r : rt) : iProp Σ :=
+    ∃ (l : loc) (ty : sigT type), ⌜static_is_registered name l ty⌝ ∗
+      ∃ (Heq : rt = projT1 ty),
+        (l ◁ᵥ{π} (rew Heq in #r) @ shr_ref (projT2 ty) static)%I.
+
+  Global Instance initialized_persistent {rt} (π : thread_id) (name : string) (r : rt) :
+    Persistent (initialized π name r).
+  Proof. apply _. Qed.
+
+  Global Instance initialized_intro_persistent {rt} (π : thread_id) name (r : rt) :
+    IntroPersistent (initialized π name r) (initialized π name r).
+  Proof. constructor. iIntros "#$". Qed.
+
+  (* On introduction of `initialized`, destruct it *)
+  Lemma simplify_initialized_hyp {rt} π (x : rt) name ty l
+    `{!TCFastDone (static_is_registered name l ty)} T:
+    (∃ (Heq : rt = projT1 ty), l ◁ᵥ{π} (rew Heq in #x) @ shr_ref (projT2 ty) static -∗ T)
+    ⊢ simplify_hyp (initialized π name x) T.
+  Proof.
+    unfold TCFastDone in *. destruct ty as [rt' ty].
+    iDestruct 1 as (?) "HT". subst; simpl in *.
+    iIntros "Hinit".
+    iDestruct "Hinit" as "(%l' & %ty' & %Hlook1' & %Heq & Hl)".
+    destruct ty' as (rt & ty'). subst. simpl in *.
+    repeat match goal with | H : static_is_registered _ _ _ |- _ => destruct H end.
+    simplify_eq.
+    match goal with | H : existT _ _ = existT _ _ |- _ => apply existT_inj in H end.
+    subst. iApply ("HT" with "Hl").
+  Qed.
+  Definition simplify_initialized_hyp_inst := [instance @simplify_initialized_hyp with 0%N].
+  Global Existing Instance simplify_initialized_hyp_inst.
+
+  Lemma initialized_intro {rt} π ty name l (x : rt) :
+    static_is_registered name l ty →
+    (∃ (Heq : rt = projT1 ty), l ◁ᵥ{π} (rew Heq in #x) @ shr_ref (projT2 ty) static) -∗
+    initialized π name x.
+  Proof. iIntros (?) "Hl". iExists _, _. by iFrame. Qed.
+
+  Lemma simplify_initialized_goal {rt} π (x : rt) name l ty
+    `{!TCFastDone (static_is_registered name l ty)} T:
+    (∃ (Heq : rt = projT1 ty), l ◁ᵥ{π} (rew Heq in #x) @ shr_ref (projT2 ty) static ∗ T)
+    ⊢ simplify_goal (initialized π name x) T.
+  Proof.
+    unfold TCFastDone in *. iIntros "[% [? $]]". subst.
+    iApply initialized_intro; [done..|]. by iExists _.
+  Qed.
+  Definition simplify_initialized_goal_inst := [instance @simplify_initialized_goal with 0%N].
+  Global Existing Instance simplify_initialized_goal_inst.
+
+  (** Subsumption *)
+  Definition FindInitialized (π : thread_id) (rt : Type) (name : string) :=
+    {| fic_A := rt; fic_Prop r := (initialized π name r); |}.
+  Global Instance related_to_initialized (π : thread_id) {rt} name (r : rt) :
+    RelatedTo (initialized π name r) :=
+    {| rt_fic := FindInitialized π rt name|}.
+
+  Set Printing Universes.
+  Lemma find_in_context_initialized π name rt (T : rt → iProp Σ):
+    (∃ x, initialized π name x ∗ T x)
+    ⊢ find_in_context (FindInitialized π rt name) T.
+  Proof. iDestruct 1 as (x) "[Hinit HT]". iExists _. iFrame. Qed.
+  Definition find_in_context_initialized_inst :=
+    [instance find_in_context_initialized with FICSyntactic].
+  Global Existing Instance find_in_context_initialized_inst | 1.
+
+  Lemma subsume_initialized π {rt} name (r1 r2 : rt) T:
+    (⌜r1 = r2⌝ ∗ T)
+    ⊢ subsume (initialized π name r1) (initialized π name r2) T.
+  Proof. iIntros "(-> & HT) ?". iFrame. Qed.
+  Definition subsume_initialized_inst := [instance subsume_initialized].
+  Global Existing Instance subsume_initialized_inst.
+End statics.
+Global Typeclasses Opaque initialized.
+
+(* After calling adequacy:
+    we need to create initialized things.
+    then we can provide them to the proof.
+
+   Users of initialized should unpack that hypothesis to get access to the type assignment.
+   This type assignment then allows us to call methods etc on the global variable.
+
+ *)
+
+
